\documentclass{article}
\usepackage{iftex}
\usepackage{ifthen}
\usepackage{epsfig}
\usepackage[utf8]{inputenc}
\usepackage{xcolor}
\ifPDFTeX
\usepackage{newunicodechar}
  \makeatletter
    \def\doxynewunicodechar#1#2{%
    \@tempswafalse
    \edef\nuc@tempa{\detokenize{#1}}%
    \if\relax\nuc@tempa\relax
      \nuc@emptyargerr
    \else
      \edef\@tempb{\expandafter\@car\nuc@tempa\@nil}%
      \nuc@check
      \if@tempswa
        \@namedef{u8:\nuc@tempa}{#2}%
      \fi
    \fi
  }
  \makeatother
  \doxynewunicodechar{⁻}{${}^{-}$}% Superscript minus
  \doxynewunicodechar{²}{${}^{2}$}% Superscript two
  \doxynewunicodechar{³}{${}^{3}$}% Superscript three

\fi
\pagestyle{empty}
\begin{document}
$ \pi/180 $
\pagebreak

$ 180/\pi $
\pagebreak

$ \mathbf{F}(\mathbf{x}) = \mathbf{0} $
\pagebreak

$ \alpha $
\pagebreak

$ \mathbf{F}
(\mathbf{x}) = \mathbf{0} $
\pagebreak

$ \mathbf{F}: \mathbb{R}^n \rightarrow
\mathbb{R}^n $
\pagebreak

\[
  \mathbf{JF}_{\mathbf{x}}(\mathbf{x}_k) \mathbf{h} = -\mathbf{F}(\mathbf{x}_k).
\]
\pagebreak

\[
  \mathbf{x}_{k+1} = \mathbf{x}_k + \alpha_k \mathbf{h}
\]
\pagebreak

$ \alpha_k $
\pagebreak

\[
\left\| \mathbf{JF}_{\mathbf{x}}(\mathbf{x}_k)^{-1} \mathbf{F}(\mathbf{x}_{k+1}) \right\|
\leq \left(1 - \dfrac{\alpha_k}{2}\right) \left\| \mathbf{JF}_{\mathbf{x}}(\mathbf{x}_k)^{-1}
\mathbf{F}(\mathbf{x}_k) \right\| = \left(1 - \dfrac{\alpha_k}{2} \right)
\left\| \mathbf{h}  \right\|.
\]
\pagebreak

$
\mathbf{F}(\mathbf{x}) = \mathbf{0} $
\pagebreak

$ \mathbf{F}: \mathbb{R}^n
\rightarrow \mathbb{R}^n $
\pagebreak

$ \epsilon $
\pagebreak

$ \left\| \mathbf{F}(\mathbf{x}) \right\| < \epsilon $
\pagebreak

$\alpha$
\pagebreak

$ \mathbf{F}(\mathbf{x}) $
\pagebreak

$ \mathbf{J}(\mathbf{x}) $
\pagebreak

\[
\begin{array}{c|c}
  \mathbf{c} & \mathbf{A} \\ \hline
             & \mathbf{b} \\
             & \\mathbf{b}_{e}
\end{array} \text{,}
\]
\pagebreak

$ \mathbf{A} $
\pagebreak

\[
\mathbf{A} = \begin{bmatrix}
  a_{11} & a_{12} & \dots  & a_{1s} \\
  a_{21} & a_{22} & \dots  & a_{2s} \\
  \vdots & \vdots & \ddots & \vdots \\
  a_{s1} & a_{s2} & \dots  & a
\end{bmatrix} \text{,}
\]
\pagebreak

$ \mathbf{b} $
\pagebreak

$ p $
\pagebreak

\[
  \mathbf{b} = \left[ b_1, b_2, \dots, b_s \right] \text{,}
\]
\pagebreak

$ \\mathbf{b}_{e} $
\pagebreak

$ \hat{p} $
\pagebreak

$ \hat{p} = p−1 $
\pagebreak

$ \hat{p} = p+1 $
\pagebreak

\[
  \\mathbf{b}_{e} = \left[ \hat{b}_1, \hat{b}_2, \dots, \hat{b}_s \right] \text{,}
\]
\pagebreak

$ \mathbf{c} $
\pagebreak

\[
  \mathbf{c} = \left[ c_1, c_2, \dots, c_s \right]^{\top} \text{.}
\]
\pagebreak

$ s $
\pagebreak

\[
\mathbf{A} = \begin{bmatrix}
  a_{11} & a_{12} & \dots  & a_{1s} \\
  a_{21} & a_{22} & \dots  & a_{2s} \\
  \vdots & \vdots & \ddots & \vdots \\
  a_{s1} & a_{s2} & \dots  & a_{ss}
\end{bmatrix} \text{,}
\]
\pagebreak

$ \mathbf{b}_{e} $
\pagebreak

\[
e = \sqrt{\dfrac{1}{n} \displaystyle\sum_{i=1}{n}\left(\dfrac
  {\mathbf{x} - \hat{\mathbf{x}}}
  {s c_i}
\right)^2}
\]
\pagebreak

$ \mathbf{x} $
\pagebreak

$ \hat{\mathbf{x}} $
\pagebreak

$
\hat{p} $
\pagebreak

$ \Delta t_{k+1} $
\pagebreak

$ 1 $
\pagebreak

$ e \approx Ch^{q+1} $
\pagebreak

$ 1 \approx Ch_{opt}^{q+1} $
\pagebreak

$ q = \min(p,\hat{p}) $
\pagebreak

\[
h_{opt} = h \left( \dfrac{1}{e} \right)^{\frac{1}{q+1}}
\]
\pagebreak

$ f $
\pagebreak

$ f = 0.8 $
\pagebreak

$ 0.9 $
\pagebreak

$ (0.25)^{1/(q+1)} $
\pagebreak

$ (0.38)^{1/(q+1)} $
\pagebreak

$ h $
\pagebreak

\[
h_{new} = h \min\left(f_{max}, \max\left(f_{max}, f \left(\dfrac{1}{e}\right)^{\frac{1}{q+1}}
\right) \right)
\]
\pagebreak

$ e \leq 1 $
\pagebreak

$ h_{new} $
\pagebreak

$ [0.8, 0.9] $
\pagebreak

$ f_{max} $
\pagebreak

$ [1.5, 5] $
\pagebreak

$ f_{min} $
\pagebreak

$ [0.1, 0.2] $
\pagebreak

$ k+1 $
\pagebreak

$
           \mathbf{x_{k+1}}(t_{k}+\Delta t) $
\pagebreak

$ \Delta t$
\pagebreak

$ \Delta
        t_{k+1} $
\pagebreak

$ \mathbf{F}(\mathbf{x}, \mathbf{x}^{\prime}, t)
= \mathbf{0} $
\pagebreak

$ \mathbf{K}_i $
\pagebreak

$ \mathbf{x}^{\prime} = \mathbf{f}(\mathbf{x}, t) $
\pagebreak

\[
\begin{array}{l}
\mathbf{K}_i = \mathbf{f} \left(
  \mathbf{x}_k + \Delta t \displaystyle\sum_{j=1}^{s} a_{ij} \mathbf{K}_j,
  \, t_k + c_i \Delta t
  \right), \qquad i = 1, 2, \ldots, s \\
\mathbf{x}_{k+1} = \mathbf{x}_k + \Delta t \displaystyle\sum_{j=1}^s b_j
\mathbf{K}_j \, ,
\end{array}
\]
\pagebreak

$ s$
\pagebreak

\[
\mathbf{K}_i = \mathbf{f} \left(
  \mathbf{x}_k + \Delta t \displaystyle\sum_{j=1}^{i-1} a_{ij}
  \mathbf{K}_j, \, t_k + c_i \Delta t
  \right), \qquad i = 1, 2, \ldots, s.
\]
\pagebreak

$\mathbf{F}(\mathbf{x}, \mathbf{x}^{\prime}, t) = \mathbf{0} $
\pagebreak

\[
\begin{array}{l}
\mathbf{F}_i \left(
  \mathbf{x}_k + \Delta t \displaystyle\sum_{j=1}^{i-1} a_{ij}
    \mathbf{K}_j, \, \mathbf{K}_i, \, t_k + c_i \Delta t
\right) = \mathbf{0}, \qquad i = 1, 2, \ldots, s \\
\mathbf{x}_{k+1} = \mathbf{x}_k + \displaystyle\sum_{j=1}^s b_j \mathbf{K}_j.
\end{array}
\]
\pagebreak

$ \mathbf{F}_i $
\pagebreak

$ \mathbf{K}
$
\pagebreak

\[
\left\{\begin{array}{l}
\mathbf{F}_1 \left(
  \mathbf{x}_k, \, \mathbf{K}_1, \, t_k + c_1 \Delta t
\right) = \mathbf{0} \\
\mathbf{F}_2 \left(
  \mathbf{x}_k + \Delta t \, a_{21} \mathbf{K}_1, \,
  \mathbf{K}_2, \, t_k + c_2 \Delta t
\right) = \mathbf{0} \\
~~ \vdots \\
\mathbf{F}_s \left(
  \mathbf{x}_k + \Delta t \displaystyle\sum_{j=1}^{s-1} a_{sj}
  \mathbf{K}_j, \, \mathbf{K}_s, \, t_k + c_s \Delta t
\right) = \mathbf{0}
\end{array}\right.
\]
\pagebreak

$ \Delta t $
\pagebreak

$ k $
\pagebreak

$ \mathbf{x}(t_k) $
\pagebreak

$ t_k $
\pagebreak

$ \mathbf{x_{k+1}}(t_{k}+\Delta t) $
\pagebreak

\[
\mathbf{F}_i\left(\mathbf{x}_k + \Delta t \displaystyle\sum_{j=1}^{s}
  a_{ij} \mathbf{K}_j, \, \mathbf{K}_i, \, t_k + c_i \Delta t
\right) = \mathbf{0}.
\]
\pagebreak

$ \mathbf{K} $
\pagebreak

\[
\mathbf{F}_i\left(\mathbf{x}_k + \Delta t \displaystyle\sum_{j=1}^s
  a_{ij} \mathbf{K}_j, \, \mathbf{K}_i, \, t_k + c_i \Delta t
\right) = \mathbf{0}
\]
\pagebreak

\[
\dfrac{\partial \mathbf{F}_i}{\partial \mathbf{K}_i} \left(
  \mathbf{x}_k + \Delta t \displaystyle\sum_{j=1}^s a_{ij} \mathbf{K}_j,
  \, \mathbf{K}_i, \, t_k + c_i \Delta t
\right)
\]
\pagebreak

$ \mathbf{F}(\mathbf{x}, \mathbf{x}^{\prime}, t) =
\mathbf{0} $
\pagebreak

$ \mathbf{x}^{\prime} = \mathbf{f}(\mathbf{x}, \mathbf{v}, t) $
\pagebreak

\[
\begin{array}{l}
\mathbf{K}_i = \mathbf{f} \left(
  \mathbf{x}_k + \Delta t \displaystyle\sum_{j=1}^{s} a_{ij}
  \mathbf{K}_j,
  \, t_k + c_i \Delta t
  \right), \qquad i = 1, 2, \ldots, s \\
\mathbf{x}_{k+1} = \mathbf{x}_k + \Delta t \displaystyle\sum_{j=1}^s b_j
\mathbf{K}_j \, ,
\end{array}
\]
\pagebreak

\[
\begin{array}{l}
\mathbf{F}_i \left(
  \mathbf{x}_k + \Delta t \displaystyle\sum_{j=1}^s a_{ij}
    \mathbf{K}_j, \, \mathbf{K}_i, \, t_k + c_i \Delta t
\right) = \mathbf{0}, \qquad i = 1, 2, \ldots, s \\
\mathbf{x}_{k+1} = \mathbf{x}_k + \displaystyle\sum_{j=1}^s b_j \mathbf{K}_j.
\end{array}
\]
\pagebreak

\[
\left\{\begin{array}{l}
\mathbf{F}_1 \left(
  \mathbf{x}_k + \Delta t \displaystyle\sum_{j=1}^s a_{1j}
  \mathbf{K}_j, \, \mathbf{K}_1, \, t_k + c_1 \Delta t
\right) = \mathbf{0} \\
\mathbf{F}_2 \left(
  \mathbf{x}_k + \Delta t \displaystyle\sum_{j=1}^s a_{2j}
  \mathbf{K}_j, \, \mathbf{K}_2, \, t_k + c_2 \Delta t
\right) = \mathbf{0} \\
~~ \vdots \\
\mathbf{F}_s \left(
  \mathbf{x}_k + \Delta t \displaystyle\sum_{j=1}^s a_{sj}
  \mathbf{K}_j, \, \mathbf{K}_s, \, t_k + c_s \Delta t
\right) = \mathbf{0}
\end{array}\right.
\]
\pagebreak

$ \mathbf{F}(\mathbf{x}, \mathbf{x}^{\prime}, \mathbf{v}, t) = \mathbf{0}
$
\pagebreak

\[
\mathbf{x}_{k+1}(t_{k}+\Delta t) = \mathbf{x}_k(t_{k}) +
\mathcal{S}(\mathbf{x}_k(t_k), \mathbf{x}^{\prime}_k(t_k), t_k, \Delta t)
\]
\pagebreak

$ \mathcal{S} $
\pagebreak

$ \mathbf{F}(\mathbf{x}, \mathbf{x}^{\prime}, \mathbf{v}, t) = \mathbf{0} $
\pagebreak

$ \mathcal{h}(\mathbf{x}, \mathbf{v}, t) $
\pagebreak

$ \mathbf{t} = \left[ t_0, t_1, \ldots, t_n
         \right]^T $
\pagebreak

$ \mathbf{x}(t = 0) $
\pagebreak

$ \left[(\mathrm{size}(\mathbf{x}) \times \mathrm{size}
           (\mathbf{t})\right] $
\pagebreak

$ \left[(\mathrm{size}(\mathbf{x}) \times \mathrm{size}
          (\mathbf{t})\right] $
\pagebreak

$ \mathbf{f} $
\pagebreak

$ t $
\pagebreak

$ \mathbf{F} $
\pagebreak

\[
  \mathbf{Jf}_{\mathbf{x}}(\mathbf{x}, t) =
  \dfrac{\partial\mathbf{f}(\mathbf{x}, t)}{\partial\mathbf{x}} \text{.}
\]
\pagebreak

$ \mathbf{JF}_{\mathbf{x}}(\mathbf{x}, \mathbf{x}^{\prime}, t) $
\pagebreak

$ \mathbf{x}^{\prime} $
\pagebreak

\[
  \mathbf{JF}_{\mathbf{x}}(\mathbf{x}, \mathbf{x}^{\prime}, t) =
  \dfrac{\partial\mathbf{F}(\mathbf{x}, \mathbf{x}^{\prime}, t)}{\partial\mathbf{x}} \text{.}
\]
\pagebreak

\[
  \mathbf{JF}_{\mathbf{x}^{\prime}}(\mathbf{x}, \mathbf{x}^{\prime}, t) =
  \dfrac{\partial\mathbf{F}(\mathbf{x}, \mathbf{x}^{\prime}, t)}{\partial\mathbf{x}^{\prime}} \text{.}
\]
\pagebreak

$ \mathbf{JF}_{\mathbf{x}^{\prime}}(\mathbf{x}, \mathbf{x}^{\prime}, t) $
\pagebreak

$ (\mathbf{x}, t) $
\pagebreak

$ \mathbf{f}(\mathbf{x}, t) $
\pagebreak

\[
\begin{array}{c|cccc}
    0 &   0 &   0 &   0 &   0 \\
  1/2 & 1/2 &   0 &   0 &   0 \\
  1/2 &   0 & 1/2 &   0 &   0 \\
    1 &   0 &   0 &   1 &   0 \\
  \hline
      & 1/6 & 1/3 & 1/3 & 1/6
\end{array} \text{.}
\]
\pagebreak

\end{document}
